pulse/lib/core/PulseCore.Action.fsti
@@ -191,6 +191,9 @@ val later_intro (p:slprop)
 val later_elim (p:slprop)
 : act unit Ghost emp_inames (later p ** later_credit 1) (fun _ -> p)
 
+val later_elim_timeless (p:slprop { timeless p })
+: act unit Ghost emp_inames (later p) (fun _ -> p)
+
 val buy1 ()
 : stt unit emp (fun _ -> later_credit 1)
 
